% ==============================================================
% Chapter: Appendix
% ==============================================================
\chapter{Appendix} \label{sec: Appendix}
% ==============================================================

\lipsum[1-2]

\begin{boxedlemma}{\cite{Hautus1970}.} \label{def: Lemma_1}
	The following statements are all equivalent: 
	\begin{subequations} \begin{align}
		\text{\emph{ I}. }& \text{The pair $(A, C)$ is observable} \\
		\text{\emph{ II}. }&\texttt{rank}(\begin{bmatrix} \lambda I - A^{\tran}  & C^{\tran} \end{bmatrix}^{\tran} ) = N_x,  \text{ } \forall \lambda \in \mathbb{C}; \\
		\text{\emph{ III}. }&\texttt{rank}(\begin{bmatrix} \lambda_i I - A^{\tran}  &  C^{\tran} \end{bmatrix}^{\tran}) = N_x, \text{ } \forall \lambda_i \in \sigma(A) \subset \mathbb{C}.
	\end{align}	\end{subequations}
\end{boxedlemma}

\begin{proof}
	Left to the interested reader.
\end{proof}

\lipsum[1][1-6]